src/tls/TLS.Handshake.Client.fst
@@ -5,24 +5,64 @@ open TLSConstants
 open TLSInfo
 open TLSError
 open FStar.HyperStack.ST
-open TLS.Handshake.State
+open TLS.Handshake.Machine
 
-module B = FStar.Bytes
+module B = LowStar.Buffer // not FStar.Bytes
 module CH = Parsers.ClientHello
 module E = Extensions
 module Epochs = Old.Epochs
 module HSM = HandshakeMessages
 module HMAC = Old.HMAC.UFCMA
 module KS = Old.KeySchedule
-module HSL = HandshakeLog
-module Nego = Negotiation
 module HS = FStar.HyperStack
 module H = Hashing.Spec
 
 #set-options "--admit_smt_queries true"
 
+let config_of #region (Client _ cfg _) = fst cfg
+
+// include TLS.Handshake.State
+
+val discard: bool -> ST unit
+  (requires (fun _ -> True))
+  (ensures (fun h0 _ h1 -> h0 == h1))
+let discard _ = ()
+let print s = discard (IO.debug_print_string ("HS | "^s^"\n"))
+unfold val trace: s:string -> ST unit
+  (requires (fun _ -> True))
+  (ensures (fun h0 _ h1 -> h0 == h1))
+unfold let trace = if DebugFlags.debug_HS then print else (fun _ -> ())
+
+
+/// floating; imported from State on demand
+
+// indexing to be reviewed
+val register:
+  #region:rgn -> #n:random -> Epochs.epochs region n ->
+  KS.recordInstance -> St unit
+
+let register #region #n epochs keys =
+    let ep = //? we don't have a full index yet for the epoch; reuse the one for keys??
+      let h = Negotiation.Fresh ({ Negotiation.session_nego = None }) in
+      Epochs.recordInstanceToEpoch #region #n h keys in // just coercion
+      // New Handshake does
+      // let KeySchedule.StAEInstance #id r w = keys in
+      // Epochs.recordInstanceToEpoch #hs.region #(nonce hs) h (Handshake.Secret.StAEInstance #id r w) in
+    Epochs.add_epoch epochs ep // actually extending the epochs log
+
+val export:
+  #region:rgn -> #n:random -> Epochs.epochs region n ->
+  KS.exportKey -> St unit
+
+let export #region #n epochs xk =
+  trace "exporting a key";
+  FStar.Monotonic.Seq.i_write_at_end epochs.Epochs.exporter xk
+
+
 (*** Version-agnostic messages ***)
 
+
+(*
 type btag (binderKey:(i:HMAC.binderId & bk:KS.binderKey i)) =
   HMAC.tag (HMAC.HMAC_Binder (let (|i,_|) = binderKey in i))
 
@@ -38,12 +78,14 @@ val map_ST2: 'c -> ('c -> 'a -> KS.ST0 'b) -> list 'a -> KS.ST0 (list 'b)
 let rec map_ST2 env f x = match x with
   | [] -> []
   | a::tl -> f env a :: map_ST2 env f tl
+*)
 
-private let client_Binders (hs:hs) (offer:HSM.clientHello) =
-  match Nego.resume hs.nego //$ use instead the hs.client_config
-  with
+
+(*
+let client_Binders #region (hs:t region) (offer:HSM.clientHello) =
+  match snd hs.cfg with
   | (_, []) ->
-    HSL.send hs.log (HSL.Msg (HSM.M_client_hello offer))
+    Send.send_ch hs.log (HSL.Msg (HSM.M_client_hello offer))
   | (_, pskl) ->
     let binderKeys = KS.ks_client13_get_binder_keys hs.ks pskl in
     let blen = E.bindersLen offer.CH.extensions in
@@ -53,131 +95,182 @@ private let client_Binders (hs:hs) (offer:HSM.clientHello) =
     HSL.send_raw hs.log bb;
 
     // Nego ensures that EDI is not sent in a 2nd ClientHello
-    if Nego.find_early_data offer then
-     begin
-      trace "setting up 0RTT";
-      let (| bid, _ |) :: _ = binderKeys in
-      let ha = binderId_hash bid in
-      let digest_CH = HSL.hash_tag #ha hs.log in
-      let early_exporter_secret, edk = KS.ks_client13_ch hs.ks digest_CH in
-      export hs early_exporter_secret;
-      register hs edk;
-      HSL.send_signals hs.log (Some (true, false)) false
-     end
+ *)
 
-let client_ClientHello hs =
+let transcript_extract #ha (di:HSL.Transcript.state ha) tx: St Bytes.bytes =
+  let ltag = EverCrypt.Hash.Incremental.hash_len ha in
+  let btag = LowStar.Buffer.alloca 0uy ltag in
+  HSL.Transcript.extract_hash di btag tx;
+  FStar.Bytes.of_buffer ltag btag
+
+/// Create a fresh transcript digest, hash the truncated client Hello,
+/// and compute the MAC for a given PSK.
+//TODO tch & logical payload
+let client_Binder region (bkey:Negotiation.bkey13) tch =
+  let ha = Negotiation.ha_bkey13 bkey in
+  let di, tx0 = HSL.Transcript.create region ha in
+  let tx1 = HSL.Transcript.extend di tch tx0 in
+  let tag = transcript_extract di tx1 in
+  let binder = KS.mk_binder #region bkey in // vs HMAC.mac bk tag, hiding tricky indexing
+  tx1, ha, di, binder
+
+let client_ClientHello (Client region config r) =
+  let (cfg,resume) = config in
+  let C_init random = !r in
   let groups =
-    match (config_of hs).max_version with
-    | TLS_1p3 ->
-      trace "offering ClientHello 1.3"; Some (config_of hs).offer_shares
-    | _ ->
-      trace "offering ClientHello 1.2"; None
-    in
-  // If groups = None, this is a 1.2 handshake
-  // Note that groups = Some [] is valid (e.g. to trigger HRR deliberately)
-  let shares = KS.ks_client_init hs.ks groups in
+    match cfg.max_version with
+    | TLS_1p3 -> trace "offering ClientHello 1.3"; Some cfg.offer_shares
+    | _       -> trace "offering ClientHello 1.2"; None in
+    // groups = None indicates a 1.2 handshake
+    // groups = Some [] is valid, may be used to deliberately trigger HRR
+  let ks, shares = KS.ks_client_init random groups in
 
   // Compute & send the ClientHello offer
-  match Nego.client_ClientHello hs.nego shares with
+  // lower: we'll instead pass the sending state for writing the offer.
+  // TODO allocate non-empty output slice!
+  let sending = Send.send_state0 in
+  match Negotiation.client_ClientHello config random shares with
   | Error z -> Error z
-  | Correct offer ->
-    // Compute and send PSK binders & 0-RTT signals
-    client_Binders hs offer;
-    // we may still need to keep parts of ch
-    hs.state := C_wait_ServerHello; //$ full_offer digest ks
-    Correct ()
+  | Correct offer0 -> (
+    let epochs = Epochs.create region random in
+    let receiving_buffer = LowStar.Buffer.alloca 0uy 12000ul in
+    let receiving = TLS.Handshake.Receive.create receiving_buffer in
 
-let client_HelloRetryRequest hs hrr =
+    // TODO: write CH, including dummy binders if it offers PSKs.
+    // Send.send_ch sending offer;
+
+    // TODO assert we have a slice with this serialized offer
+
+    // TODO: postcondition stating the transcript is at [ClientHello None offer1], and computing ha from offer1 too
+    let (| offer1, ha, digest |) : (_ & ha:_ & HSL.Transcript.state ha) = (
+      match resume with
+      | (_,[]) -> (
+        let ha = EverCrypt.Hash.Incremental.SHA2_256 in // a reasonable default
+        let di, tx0 = HSL.Transcript.create region ha in
+        let tx1 = HSL.Transcript.(extend di (admit()) (* LR_ClientHello of offer *) tx0) in
+        (| offer0, ha, di |) )
+
+      | (_,(psk0::psks)) -> (
+        // TODO intermediate write to hs for witnessing the binder's
+        // logical payload; this requires a dummy digest.
+        let tx1, ha, di, binder = client_Binder region psk0 (admit()) (* LR_TCH of offer *) in
+        // TODO iterate on the other binders [psks], deallocating their auxiliary digests
+        // TODO patch both the offer and its serialization in [sending]
+        let offer1 = offer0 in
+        let tx2 = HSL.Transcript.(extend di (admit()) (* LR_CompleteTCH of [binder] *) tx1) in
+        let sending =
+        if Negotiation.find_early_data offer0 then (
+          trace "setting up 0RTT";
+          let digest_CH = transcript_extract di tx2  in
+          // TODO consider doing export & register within KS
+          let early_exporter_secret, edk = KS.ks_client13_ch cfg.is_quic ks digest_CH in
+          export epochs early_exporter_secret;
+          register epochs edk;
+          Send.signals sending (Some (true, false)) false )
+        else sending in
+        (| offer1, ha, di |))) in
+
+    let ms: msg_state region ParseFlights.F_c_wait_ServerHello random ha = {
+      digest = digest;
+      sending = sending;
+      receiving = receiving;
+      epochs = epochs;
+    } in
+    r := C_wait_ServerHello ({full_retry=None; full_ch=offer1}) ms ks;
+    Correct () )
+
+let client_HelloRetryRequest (Client region config r) hrr =
   trace "client_HelloRetryRequest";
-  let s =
-    match Nego.group_of_hrr hrr with
+  let C_wait_ServerHello offer ms ks = !r in
+  let share, ks =
+    match Negotiation.group_of_hrr hrr with
     | None ->
       // this case should only ever happen in QUIC stateless retry address validation
       // FIXME(adl) deprecated in current QUIC with transport retry
-      trace "Server did not specify a group in HRR, re-using the previous choice"; None
+      trace "Server did not specify a group in HRR, re-using the previous choice"; None, ks
     | Some ng ->
         let Some g = CommonDH.group_of_namedGroup ng in
-        let s = KS.ks_client13_hello_retry hs.ks g in
-        Some (| g, s |)
+        let s, ks = KS.ks_client13_hello_retry ks g in
+        Some (| g, s |), ks
     in
-  match Nego.client_HelloRetryRequest hs.nego hrr s with
-  | Error z -> InError z
-  | Correct(ch) ->
-    client_Binders hs ch;
-    // Note: we stay in Wait_ServerHello
-    // Only the Nego state machine was moved by HRR
-    InAck false false
+  match Negotiation.client_HelloRetryRequest offer.full_ch hrr share with
+  | Error z -> Receive.InError z
+  | Correct offer2 -> (
+    // TODO: adapt from the code above
+    // does it make sense to send binders with the wrong hash algorithm?
 
-let client_ServerHello s sh =
+    // WAS: (assuming the server's required share had already been sent)
+    // client_Binders hs ch2;
+    // // Note: we stay in Wait_ServerHello
+    // // Only the Nego state machine was moved by HRR
+    Receive.InAck false false )
+
+let client_ServerHello (Client region config r) sh =
   trace "client_ServerHello";
-  match Nego.client_ServerHello s.nego sh with
-  | Error z -> InError z
-  | Correct mode ->
-    let pv = mode.Nego.n_protocol_version in
-    let cfg = Nego.local_config s.nego in
-    let ha = Nego.hashAlg mode in
-    let ka = Nego.kexAlg mode in
-    HandshakeLog.setParams s.log pv ha (Some ka) None (*?*);
-    match pv with
-    | TLS_1p3 ->
-      begin
-        trace "Running TLS 1.3";
-        let digest_ServerHello = HSL.hash_tag #ha s.log in
-        let hs_keys = KS.ks_client13_sh s.ks
-          mode.Nego.n_server_random
-          mode.Nego.n_cipher_suite
-          digest_ServerHello
-          mode.Nego.n_server_share
-          mode.Nego.n_pski in
-        register s hs_keys; // register new epoch
-        if Nego.zeroRTToffer mode.Nego.n_offer then
-         begin
-          // Skip the 0-RTT epoch on the reading side
-          Epochs.incr_reader s.epochs;
-          match mode.Nego.n_pski with
-          | None ->
-            trace "0-RTT rejected early (no PSK was selected)";
-            Epochs.incr_writer s.epochs
-          | Some _ ->
-            trace "0RTT potentially accepted (wait for EE to confirm)";
-            // No EOED in QUIC, so we immediately enable HSK
-            if cfg.is_quic then Epochs.incr_writer s.epochs
-         end
-        else // No EOED to send in 0-RTT epoch
-          Epochs.incr_writer s.epochs; // Next flight (CFin) will use HSK
-        s.state := C13_wait_Finished1;
-        Epochs.incr_reader s.epochs; // Client 1.3 HSK switch to handshake key for decrypting EE etc...
-        InAck true false // Client 1.3 HSK
-      end
-    | _ ->
-      begin
-        trace "Running classic TLS";
-        trace ("Offered SID="^(B.print_bytes mode.Nego.n_offer.CH.session_id)^" Server SID="^(B.print_bytes mode.Nego.n_sessionID));
-        if Nego.resume_12 mode then
-         begin // 1.2 resumption
-          trace "Server accepted our 1.2 ticket.";
-          let Some (tid, Ticket.Ticket12 pv cs ems msId ms) = fst (Nego.resume s.nego) in
-          let pv' = mode.Nego.n_protocol_version in
-          let cs' = mode.Nego.n_cipher_suite in
-          let sr = mode.Nego.n_server_random in
-          let nst = Nego.sendticket_12 mode in
-          if pv = pv' && cs = cs' then // TODO check full session
-           begin
-            let adk = KS.ks_client12_resume s.ks sr pv cs ems msId ms in
-            let digestSH = HSL.hash_tag #ha s.log in
-            register s adk;
-            s.state := (if nst then C_wait_NST true else C_wait_CCS (true, digestSH));
-            InAck false false
-           end
-          else
-            InError (fatalAlert Handshake_failure, "inconsistent protocol version or ciphersuite during resumption")
-         end
+  let cfg,_ = config in
+  let C_wait_ServerHello offer ms ks = !r in
+  match Negotiation.client_accept_ServerHello config offer.full_ch sh with
+  | Error z -> Receive.InError z
+  | Correct (cs,pski) -> (
+    match cs with
+    | CipherSuite13 ae ha -> (
+      trace "Running TLS 1.3";
+      let server_share = Negotiation.find_serverKeyShare sh in
+      let digest_ServerHello = HSL.hash_tag #ha s.log in
+      let hs_keys, ks = KS.ks_client13_sh
+        s.ks
+        cfg.is_quic
+        sh.RealServerHello.random
+        (CipherSuite13 ae ha)
+        digest_ServerHello
+        server_share
+        pski in
+      register sms.epochs hs_keys; // register new epoch
+      if Negotiation.zeroRTToffer offer.full_ch then (
+        // Skip the 0-RTT epoch on the reading side
+        Epochs.incr_reader s.epochs;
+        match mode.Negotiation.n_pski with
+        | None ->
+          trace "0-RTT rejected early (no PSK was selected)";
+          Epochs.incr_writer s.epochs
+        | Some _ ->
+          trace "0RTT potentially accepted (wait for EE to confirm)";
+          // No EOED in QUIC, so we immediately enable HSK
+          if cfg.is_quic then Epochs.incr_writer ms.epochs )
+      else // No EOED to send in 0-RTT epoch
+        Epochs.incr_writer ms.epochs; // Next flight (CFin) will use HSK
+
+      Epochs.incr_reader ms.epochs; // Client 1.3 HSK switch to handshake key for decrypting EE etc...
+      r := C13_wait_Finished1 offer sh ms ks;
+      Receive.InAck true false // Client 1.3 HSK
+    )
+    | CipherSuite kex sa ae -> (
+      trace "Running classic TLS";
+      trace ("Offered SID="^(Bytes.print_bytes mode.Negotiation.n_offer.CH.session_id)^" Server SID="^(Bytes.print_bytes mode.Negotiation.n_sessionID));
+      if Negotiation.resume_12 mode then
+      begin // 1.2 resumption
+        trace "Server accepted our 1.2 ticket.";
+        let Some (tid, Ticket.Ticket12 pv cs ems msId ms) = fst (Negotiation.resume s.nego) in
+        let pv' = mode.Negotiation.n_protocol_version in
+        let cs' = mode.Negotiation.n_cipher_suite in
+        let sr = mode.Negotiation.n_server_random in
+        let nst = Negotiation.sendticket_12 mode in
+        if pv = pv' && cs = cs' then // TODO check full session
+        begin
+          let adk = KS.ks_client12_resume s.ks sr pv cs ems msId ms in
+          let digestSH = HSL.hash_tag #ha s.log in
+          register s adk;
+          s.state := (if nst then C_wait_NST true else C_wait_CCS (true, digestSH));
+          InAck false false
+        end
         else
-         begin // 1.2 full handshake
-           s.state := C_wait_ServerHelloDone;
-           InAck false false
-         end
+          InError (fatalAlert Handshake_failure, "inconsistent protocol version or ciphersuite during resumption")
       end
+      else
+      begin // 1.2 full handshake
+        s.state := C_wait_ServerHelloDone;
+        InAck false false
+      end ))
 
 (*** TLS 1.2 ***)
 
@@ -189,14 +282,14 @@ private let convert_kex = function
 
 let client_ServerHelloDone hs c ske_bytes ocr =
   trace "processing ...ServerHelloDone";
-  let kex = Nego.kexAlg (Nego.getMode hs.nego) in
+  let kex = Negotiation.kexAlg (Negotiation.getMode hs.nego) in
   match convert_kex kex with
   | Error z -> InError z
   | Correct kex ->
   match HSM.serverKeyExchange_parser32 kex ske_bytes with
   | None -> InError (fatalAlert Decode_error, "invalid client key exchange")
   | Some (ske, _) ->
-  match Nego.client_ServerKeyExchange hs.nego c kex ske ocr with
+  match Negotiation.client_ServerKeyExchange hs.nego c kex ske ocr with
   | Error z -> InError z
   | Correct mode -> (
     (match ocr with
@@ -204,14 +297,14 @@ let client_ServerHelloDone hs c ske_bytes ocr =
     | Some cr ->
       trace "processing certificate request (TODO)";
       HSL.send hs.log (HSL.Msg12 (HSM.M12_certificate [])));
-    let nst = Nego.sendticket_12 mode in
-    let gy = Some?.v (mode.Nego.n_server_share) in // already set in KS
+    let nst = Negotiation.sendticket_12 mode in
+    let gy = Some?.v (mode.Negotiation.n_server_share) in // already set in KS
     let gx =
       KS.ks_client12_full_dh hs.ks
-      mode.Nego.n_server_random
-      mode.Nego.n_protocol_version
-      mode.Nego.n_cipher_suite
-      (Nego.emsFlag mode) // a flag controlling the use of ems
+      mode.Negotiation.n_server_random
+      mode.Negotiation.n_protocol_version
+      mode.Negotiation.n_cipher_suite
+      (Negotiation.emsFlag mode) // a flag controlling the use of ems
       gy in
     let (|g, _|) = gy in
     let gxb = CommonDH.serialize_raw gx in
@@ -222,7 +315,7 @@ let client_ServerHelloDone hs c ske_bytes ocr =
       | HSM.Dhe -> Cke_dhe gxb in
     let msg = HSM.M12_client_key_exchange (
       clientKeyExchange_serializer32 kex cke) in
-    let ha = verifyDataHashAlg_of_ciphersuite (mode.Nego.n_cipher_suite) in
+    let ha = verifyDataHashAlg_of_ciphersuite (mode.Negotiation.n_cipher_suite) in
     let digestClientKeyExchange = HSL.send_tag #ha hs.log (HSL.Msg12 msg) in
     let cfin_key, app_keys = KS.ks_client12_set_session_hash hs.ks digestClientKeyExchange in
     register hs app_keys;
@@ -240,8 +333,8 @@ let client_ServerHelloDone hs c ske_bytes ocr =
 let client_R_ServerFinished hs f digestNewSessionTicket digestServerFinished =
   trace "client_R_ServerFinished";
   let sfin_key = KS.ks12_finished_key hs.ks in
-  let mode = Nego.getMode hs.nego in
-  let ha = verifyDataHashAlg_of_ciphersuite mode.Nego.n_cipher_suite in
+  let mode = Negotiation.getMode hs.nego in
+  let ha = verifyDataHashAlg_of_ciphersuite mode.Negotiation.n_cipher_suite in
   let expected_svd = TLSPRF.finished12 ha sfin_key Server digestNewSessionTicket in
   if f = expected_svd
   then (
@@ -251,39 +344,39 @@ let client_R_ServerFinished hs f digestNewSessionTicket digestServerFinished =
     InAck false false // send_CCS_tag buffers the complete
   )
   else
-    InError (fatalAlert Decode_error, "Finished MAC did not verify: expected digest "^B.print_bytes digestNewSessionTicket)
+    InError (fatalAlert Decode_error, "Finished MAC did not verify: expected digest "^Bytes.print_bytes digestNewSessionTicket)
 
 let client_ServerFinished hs f digestClientFinished =
   let sfin_key = KS.ks12_finished_key hs.ks in
-  let mode = Nego.getMode hs.nego in
-  let ha = verifyDataHashAlg_of_ciphersuite mode.Nego.n_cipher_suite in
+  let mode = Negotiation.getMode hs.nego in
+  let ha = verifyDataHashAlg_of_ciphersuite mode.Negotiation.n_cipher_suite in
   let expected_svd = TLSPRF.finished12 ha sfin_key Server digestClientFinished in
-  //let expected_svd = TLSPRF.verifyData (mode.Nego.n_protocol_version,mode.Nego.n_cipher_suite) sfin_key Server digestClientFinished in
+  //let expected_svd = TLSPRF.verifyData (mode.Negotiation.n_protocol_version,mode.Negotiation.n_cipher_suite) sfin_key Server digestClientFinished in
   if f = expected_svd
   then (
     hs.state := C_Complete; // ADL: TODO need a proper renego state Idle (Some (vd,svd)))};
     InAck false true // Client 1.2 ATK
     )
   else
-    InError (fatalAlert Decode_error, "Finished MAC did not verify: expected digest "^B.print_bytes digestClientFinished)
+    InError (fatalAlert Decode_error, "Finished MAC did not verify: expected digest "^Bytes.print_bytes digestClientFinished)
 
 let client_NewSessionTicket_12 (hs:hs) (resume:bool) (digest:Hashing.anyTag) (st: HSM.newSessionTicket12)
   : St incoming =
   let open Parsers.NewSessionTicket12 in
   let open TLS.Callbacks in
-  trace ("Processing ticket: "^B.print_bytes st.ticket);
+  trace ("Processing ticket: "^Bytes.print_bytes st.ticket);
 
   hs.state := C_wait_CCS (resume, digest);
-  let cfg = Nego.local_config hs.nego in
+  let cfg = Negotiation.local_config hs.nego in
   let tcb = cfg.ticket_callback in
-  let mode = Nego.getMode hs.nego in
-  let Some sni = B.iutf8_opt (Nego.get_sni mode.Nego.n_offer) in
+  let mode = Negotiation.getMode hs.nego in
+  let Some sni = Bytes.iutf8_opt (Negotiation.get_sni mode.Negotiation.n_offer) in
 
   let (_msId, ms) = KS.ks12_ms hs.ks in
   let info = TLS.Callbacks.TicketInfo_12 (
-    mode.Nego.n_protocol_version,
-    mode.Nego.n_cipher_suite,
-    Nego.emsFlag mode) in
+    mode.Negotiation.n_protocol_version,
+    mode.Negotiation.n_cipher_suite,
+    Negotiation.emsFlag mode) in
 
   tcb.new_ticket tcb.ticket_context sni st.ticket info ms;
   InAck false false
@@ -291,13 +384,13 @@ let client_NewSessionTicket_12 (hs:hs) (resume:bool) (digest:Hashing.anyTag) (st
 (*** TLS 1.3 ***)
 
 let client_ClientFinished_13 hs digestServerFinished ocr cfin_key =
-  let mode = Nego.getMode hs.nego in
-  let ha = verifyDataHashAlg_of_ciphersuite (mode.Nego.n_cipher_suite) in
+  let mode = Negotiation.getMode hs.nego in
+  let ha = verifyDataHashAlg_of_ciphersuite (mode.Negotiation.n_cipher_suite) in
   let digest =
     match ocr with
     | Some cr ->
       let open Parsers.Certificate13 in
-      let c = ({certificate_request_context = B.empty_bytes; certificate_list = []}) in
+      let c = ({certificate_request_context = Bytes.empty_bytes; certificate_list = []}) in
       HandshakeLog.send_tag #ha hs.log (HSL.Msg13 (HSM.M13_certificate c))
     | None -> digestServerFinished in
   let (| finId, cfin_key |) = cfin_key in
@@ -313,8 +406,8 @@ let client_ServerFinished_13 hs ee ocr oc ocv
   let oc =
     let open Parsers.Certificate13 in
     match oc with | None -> None | Some c -> Some c.certificate_list in
-  let cfg = Nego.local_config hs.nego in
-  match Nego.clientComplete_13 hs.nego ee ocr oc ocv digestCert with
+  let cfg = Negotiation.local_config hs.nego in
+  match Negotiation.clientComplete_13 hs.nego ee ocr oc ocv digestCert with
   | Error z -> InError z
   | Correct mode ->
     // ADL: 4th returned value is the exporter master secret.
@@ -322,17 +415,17 @@ let client_ServerFinished_13 hs ee ocr oc ocv
        let (sfin_key, cfin_key, app_keys, exporter_master_secret) = KS.ks_client13_sf hs.ks digestServerFinished in
        let (| finId, sfin_key |) = sfin_key in
        if not (HMAC.verify sfin_key digestCertVerify svd)
-       then InError (fatalAlert Decode_error, "Finished MAC did not verify: expected digest "^B.print_bytes digestCertVerify )
+       then InError (fatalAlert Decode_error, "Finished MAC did not verify: expected digest "^Bytes.print_bytes digestCertVerify )
        else
        begin
          export hs exporter_master_secret;
          register hs app_keys; // ATKs are ready to use in both directions
 
          // EOED emitting (not used for QUIC)
-         if Nego.zeroRTT mode && not cfg.is_quic then
+         if Negotiation.zeroRTT mode && not cfg.is_quic then
          begin
            trace "Early data accepted; emitting EOED.";
-           let ha = Nego.hashAlg mode in
+           let ha = Negotiation.hashAlg mode in
            let digestEOED = HSL.send_tag #ha hs.log (HSL.Msg13 (HSM.M13_end_of_early_data ())) in
            HSL.send_signals hs.log (Some (false, false)) false;
            hs.state := C13_sent_EOED digestEOED ocr cfin_key;
@@ -340,41 +433,42 @@ let client_ServerFinished_13 hs ee ocr oc ocv
          end
          else
          begin
-           (if Nego.zeroRTT mode then trace "Early data accepted (QUIC, no EOED)."
+           (if Negotiation.zeroRTT mode then trace "Early data accepted (QUIC, no EOED)."
            else trace "Early data rejected");
            client_ClientFinished_13 hs digestServerFinished ocr cfin_key;
            InAck true false // Client 1.3 ATK; next the client will read again to send Finished, writer++, and the Complete signal
          end
        end // moving to C_Complete
 
-let client_NewSessionTicket_13 hs st13 =
+let c13_NewSessionTicket hs st13 =
   let open TLS.Callbacks in
   let open Parsers.NewSessionTicket13 in
   let open Parsers.NewSessionTicketExtension in
   let tid = st13.ticket in
   let nonce = st13.ticket_nonce in
   let age_add = st13.ticket_age_add in
-  trace ("Received ticket: "^(B.hex_of_bytes tid)^" nonce: "^(B.hex_of_bytes nonce));
-  let mode = Nego.getMode hs.nego in
-  let CipherSuite13 ae h = mode.Nego.n_cipher_suite in
-  let ed = List.Tot.find NSTE_early_data? st13.extensions in
+  trace ("Received ticket: "^Bytes.hex_of_bytes tid^" nonce: "^Bytes.hex_of_bytes nonce);
 
-  let now = UInt32.uint_to_t (FStar.Date.secondsFromDawn()) in
-  let info = TicketInfo_13 TLS.Callbacks.({
-    ticket_nonce = Some nonce;
-    time_created = now;
-    ticket_age_add = age_add;
-    allow_early_data = Some? ed;
-    allow_dhe_resumption = true;
-    allow_psk_resumption = true;
-    early_cs = mode.Nego.n_cipher_suite;
-    identities = (B.empty_bytes, B.empty_bytes); // TODO certs
-  }) in
+  match !hs.state with
+  | C13_complete offer sh ee server_id _fin1 _fin2 _eoed_args _ms ks ->
+    let cs = sh.RealServerHello.cipher_suite in
+    let ed = List.Tot.find NSTE_early_data? st13.extensions in
+    let now = UInt32.uint_to_t (FStar.Date.secondsFromDawn()) in
+    let info = TicketInfo_13 TLS.Callbacks.({
+      ticket_nonce = Some nonce;
+      time_created = now;
+      ticket_age_add = age_add;
+      allow_early_data = Some? ed;
+      allow_dhe_resumption = true;
+      allow_psk_resumption = true;
+      early_cs = cs;
+      identities = (Bytes.empty_bytes, Bytes.empty_bytes); // TODO certs
+    }) in
 
-  let psk = KS.ks_client13_rms_psk hs.ks nonce in
-  let Some sni = B.iutf8_opt (Nego.get_sni mode.Nego.n_offer) in
-  let cfg = Nego.local_config hs.nego in
-  let valid_ed =
+    let psk = KS.ks_client13_rms_psk ks nonce in
+    let Some sni = Bytes.iutf8_opt (Negotiation.get_sni offer.full_ch) in
+    let cfg = fst hs.cfg in
+    let valid_ed =
     if cfg.is_quic then
       (match ed with
       | None -> true
@@ -387,3 +481,12 @@ let client_NewSessionTicket_13 hs st13 =
     InAck false false)
   else
     InError (fatalAlert Illegal_parameter, "QUIC tickets must allow 0xFFFFFFFF bytes of early data")
+
+
+let early_rejected st =
+  match !st.cstate with
+  | C13_wait_Finished1 offer sh _ _
+  | C13_complete offer sh _ _ _ _ _ _ _ ->
+    Negotiation.find_early_data offer.full_ch &&
+    not (List.Tot.existb SHE_early_data? sh.Parsers.RealServerHello.extensions)
+  | _ -> false
