src/tls/TLS.Handshake.Client.fsti
@@ -4,9 +4,9 @@ open Mem
 open TLSConstants
 open TLSError
 open FStar.HyperStack.ST
-open TLS.Handshake.State
+open TLS.Handshake.Machine
 
-module B = FStar.Bytes
+module B = LowStar.Buffer // not FStar.Bytes
 module CH = Parsers.ClientHello
 module HSM = HandshakeMessages
 module HMAC = Old.HMAC.UFCMA
@@ -16,17 +16,26 @@ module Nego = Negotiation
 module HS = FStar.HyperStack
 module H = Hashing.Spec
 
+(*** Hello messages ***)
+
+let inv (Client rgn cfg st:client) h0 =
+  h0 `HS.contains` st /\
+  B.loc_disjoint (B.loc_mreference st) (TLS.Handshake.Machine.client_footprint (HS.sel h0 st)) /\
+  TLS.Handshake.Machine.client_invariant (HS.sel h0 st) h0
+
+/// C_Init ==> C_wait_ServerHello
 val client_ClientHello:
-  s:hs ->
+  hs: client ->
   ST (result unit)
   (requires fun h0 ->
-    let n = HS.sel h0 Nego.(s.nego.state) in
-    let t = HSL.transcript h0 s.log in
-    let k = HS.sel h0 s.ks.KS.state in
-    match n with
-    | Nego.C_Init nonce -> k = KS.(C (C_Init nonce)) /\ t = []
-    | _ -> False )
+    inv hs h0 /\ (
+    match hs with
+    | Client _ _ r -> C_init? (HS.sel h0 r)))
   (ensures fun h0 r h1 ->
+    // see precise post-condition in the stateful invariant
+    inv hs h1)
+
+(*
     let n = HS.sel h0 Nego.(s.nego.state) in
     let t = HSL.transcript h0 s.log in
     let k = HS.sel h1 s.ks.KS.state in
@@ -46,72 +55,118 @@ val client_ClientHello:
             else k = KS.(C(C12_Full_CH offer.CH.random)) /\
           t = [HSL.Msg (HSM.M_client_hello offer)] ))
         | _ -> False )))
+*)
 
 val client_HelloRetryRequest:
-  hs: hs ->
+  hs: client ->
   hrr: HSM.hrr ->
-  St incoming
+  ST Receive.incoming
+  (requires fun h0 ->
+    inv hs h0 /\ (
+    match hs with
+    | Client _ _ r -> C_wait_ServerHello? (HS.sel h0 r)))
+  (ensures fun h0 r h1 ->
+    inv hs h1)
+
+(* useless?
+let client_sel_t (Client rgn cfg r:client) = client_state rgn cfg
+let client_sel h c: GTot (client_sel_t c) =
+  let Client rgn cfg r = c in
+  HS.sel h r
+*)
 
 val client_ServerHello:
-  hs: hs ->
+  hs: client ->
   sh: HSM.sh ->
-  St incoming
+  ST Receive.incoming
+  (requires fun h0 ->
+    let Client rgn cfg r = hs in
+    inv hs h0 /\
+    C_wait_ServerHello? (HS.sel h0 r))
+  (ensures fun h0 r h1 ->
+    inv hs h1)
+
 
 (*** TLS 1.2 ***)
 
 val client_ServerHelloDone:
-  hs ->
+  hs: client ->
   cert: HSM.certificate12 ->
-  ske_bytes: B.bytes -> // delayed parsing
+  ske_bytes: Bytes.bytes -> // delayed parsing
   cr: option HSM.certificateRequest12 ->
-  ST incoming
-  (requires (fun h -> True))
-  (ensures (fun h0 i h1 -> True))
+  ST Receive.incoming
+  (requires fun h0 -> inv hs h0)
+  (ensures fun h0 i h1 -> inv hs h1)
 
 val client_R_ServerFinished:
-  hs: hs ->
-  f: B.bytes ->
+  hs: client ->
+  f: Bytes.bytes ->
   digest_nst: H.anyTag ->
   digest_sf: H.anyTag ->
-  St incoming
+  ST Receive.incoming
+  (requires fun h0 -> inv hs h0)
+  (ensures fun h0 i h1 -> inv hs h1)
 
 val client_ServerFinished:
-  hs: hs ->
-  fin: B.bytes ->
+  hs: client ->
+  fin: Bytes.bytes ->
   digest: H.anyTag ->
-  St incoming
+  ST Receive.incoming
+  (requires fun h0 -> inv hs h0)
+  (ensures fun h0 i h1 -> inv hs h1)
 
 val client_NewSessionTicket_12:
-  hs: hs ->
+  hs: client ->
   resume: bool ->
   digest: H.anyTag ->
   nst: HSM.newSessionTicket12 ->
-  St incoming
+  ST Receive.incoming
+  (requires fun h0 -> inv hs h0)
+  (ensures fun h0 i h1 -> inv hs h1)
 
 (*** TLS 1.3 ***)
 
+/// process the TLS 1.3 decrypted server flight
+/// EncryptedExtension...ServerFinished
+///
+val c13_Finished1:
+  hs: client ->
+  ee: HSM.encryptedExtensions ->
+  ocr: option HSM.certificateRequest13 ->
+  oc: option HSM.certificate13 ->
+  ocv: option HSM.certificateVerify13 ->
+  svd: Bytes.bytes ->
+  digestCert: option H.anyTag ->
+  digestCertVerify: H.anyTag ->
+  digestServerFinished: H.anyTag ->
+  ST Receive.incoming
+  (requires fun h0 ->
+    let Client _ _ r = hs in
+    inv hs h0 /\
+    C13_wait_Finished1? (HS.sel h0 r))
+  (ensures fun h0 i h1 -> inv hs h1)
+
 // Send ClientFinished flight (hide from API?)
 val client_ClientFinished_13:
-  hs: hs ->
+  hs: client ->
   digest: H.anyTag ->
   cr: option HSM.certificateRequest13 ->
   cfk: (i:HMAC.finishedId & cfk:KS.fink i) ->
   St unit
 
-(* receive EncryptedExtension...ServerFinished for TLS 1.3, roughly mirroring client_ServerHelloDone *)
-val client_ServerFinished_13:
-  s: hs ->
-  ee: HSM.encryptedExtensions ->
-  ocr: option HSM.certificateRequest13 ->
-  oc: option HSM.certificate13 ->
-  ocv: option HSM.certificateVerify13 ->
-  svd: B.bytes ->
-  digestCert: option H.anyTag ->
-  digestCertVerify: H.anyTag ->
-  digestServerFinished: H.anyTag ->
-  St incoming
-
-val client_NewSessionTicket_13:
-  hs: hs ->
+val c13_NewSessionTicket:
+  hs: client ->
   nst: HSM.newSessionTicket13 ->
-  St incoming
+  ST Receive.incoming
+  (requires fun h0 ->
+    let Client _ _ r = hs in
+    inv hs h0 /\
+    C13_complete? (HS.sel h0 r))
+  (ensures fun h0 i h1 -> inv hs h1)
+
+// used for QUIC signalling; underspecified
+val early_rejected:
+  hs: client ->
+  ST bool
+  (requires fun h0 -> inv hs h0)
+  (ensures fun h0 r h1 -> h0 == h1)
